06GroupedEnvironments/VariableSplitting.thy
@@ -1,0 +1,363 @@
+theory VariableSplitting
+  imports GroupedEnvironments "../05Closure/Closure"
+begin
+
+section \<open>Variable splitting\<close>
+
+text \<open>Now we divide our variables into frame-offset pairs. The process is quite simple for 
+expressions: we accumulate a map from Debruijn indices to frame-offset pairs, adding to it every 
+time we pass a binder, and then map variables when we reach them. (As mentioned before, we also 
+record the frame-size every time we reach a \<open>Lam\<^sub>d\<close>.\<close>
+
+abbreviation map_past_lam :: "(nat \<rightharpoonup> nat \<times> nat) \<Rightarrow> nat \<rightharpoonup> nat \<times> nat" where
+  "map_past_lam \<Phi> x \<equiv> (case x of 
+      0 \<Rightarrow> Some (0, 0) 
+    | Suc x \<Rightarrow> map_option (apfst Suc) (\<Phi> x))"
+
+abbreviation map_past_let :: "(nat \<rightharpoonup> nat \<times> nat) \<Rightarrow> nat \<rightharpoonup> nat \<times> nat" where
+  "map_past_let \<Phi> x \<equiv> (case x of 
+      0 \<Rightarrow> Some (0, 0) 
+    | Suc x \<Rightarrow> map_option (\<lambda>(y, z). (y, if y = 0 then Suc z else z)) (\<Phi> x))"
+
+primrec split_vars' :: "(nat \<rightharpoonup> nat \<times> nat) \<Rightarrow> expr\<^sub>d \<Rightarrow> expr\<^sub>g" where
+  "split_vars' \<Phi> (Var\<^sub>d x) = (case the (\<Phi> x) of (y, z) \<Rightarrow> Var\<^sub>g y z)"
+| "split_vars' \<Phi> (Const\<^sub>d n) = Const\<^sub>g n"
+| "split_vars' \<Phi> (Lam\<^sub>d t e) = (let e\<^sub>g = split_vars' (map_past_lam \<Phi>) e in Lam\<^sub>g t e\<^sub>g (let_count e\<^sub>g))"
+| "split_vars' \<Phi> (App\<^sub>d e\<^sub>1 e\<^sub>2) = App\<^sub>g (split_vars' \<Phi> e\<^sub>1) (split_vars' \<Phi> e\<^sub>2)"
+| "split_vars' \<Phi> (Let\<^sub>d e\<^sub>1 e\<^sub>2) = Let\<^sub>g (split_vars' \<Phi> e\<^sub>1) (split_vars' (map_past_let \<Phi>) e\<^sub>2)"
+
+definition split_vars :: "expr\<^sub>d \<Rightarrow> expr\<^sub>g" where
+  "split_vars e \<equiv> split_vars' Map.empty e"
+
+text \<open>The problem arises when we try to map closures (and, for the same reason, the callstack). We 
+have an environment and an expression to be evaluated in that environment; we need to split the 
+environment up somehow. But the closure is contextless: unlike an expression, which sits within a 
+larger expression from which we can determine the structure of its environment, a closure's 
+environment is complete in itself, and provides no information about how it was constructed. 
+The same closure could group to multiple different legitimate grouped-environment closures. So we 
+cannot run the splitting process on the whole of the state.\<close>
+
+text \<open>Instead, we define the inverse, combining operation. First we define it on expressions:\<close>
+
+abbreviation inv_map_past_lam :: "(nat \<times> nat \<rightharpoonup> nat) \<Rightarrow> nat \<times> nat \<rightharpoonup> nat" where
+  "inv_map_past_lam \<Phi> x \<equiv> (case x of 
+      (0, 0) \<Rightarrow> Some 0 
+    | (0, Suc z) \<Rightarrow> None
+    | (Suc y, z) \<Rightarrow> map_option Suc (\<Phi> (y, z)))"
+
+abbreviation inv_map_past_let :: "(nat \<times> nat \<rightharpoonup> nat) \<Rightarrow> nat \<times> nat \<rightharpoonup> nat" where
+  "inv_map_past_let \<Phi> x \<equiv> (case x of (y, z) \<Rightarrow> 
+      if y = 0 \<and> z = 0 then Some 0
+      else map_option Suc (\<Phi> (y, if y = 0 then z - 1 else z)))"
+
+primrec combine_vars' :: "(nat \<times> nat \<rightharpoonup> nat) \<Rightarrow> expr\<^sub>g \<Rightarrow> expr\<^sub>d" where
+  "combine_vars' \<Phi> (Var\<^sub>g x y) = Var\<^sub>d (the (\<Phi> (x, y)))"
+| "combine_vars' \<Phi> (Const\<^sub>g n) = Const\<^sub>d n"
+| "combine_vars' \<Phi> (Lam\<^sub>g t e n) = Lam\<^sub>d t (combine_vars' (inv_map_past_lam \<Phi>) e)"
+| "combine_vars' \<Phi> (App\<^sub>g e\<^sub>1 e\<^sub>2) = App\<^sub>d (combine_vars' \<Phi> e\<^sub>1) (combine_vars' \<Phi> e\<^sub>2)"
+| "combine_vars' \<Phi> (Let\<^sub>g e\<^sub>1 e\<^sub>2) = Let\<^sub>d (combine_vars' \<Phi> e\<^sub>1) (combine_vars' (inv_map_past_let \<Phi>) e\<^sub>2)"
+
+definition combine_vars :: "expr\<^sub>g \<Rightarrow> expr\<^sub>d" where
+  "combine_vars e \<equiv> combine_vars' Map.empty e"
+
+text \<open>We can prove (in \<open>combine_split_cancel\<close> and \<open>split_combine_cancel\<close>) that our two operations 
+split and combine are inverses; or at least, are inverses on closed expressions (as shown by their 
+typechecking in the empty context).\<close>
+
+lemma inv_map_past_lam_inv [simp]: "(\<And>x y. \<Phi> x = Some y \<Longrightarrow> \<Phi>' y = Some x) \<Longrightarrow> 
+    map_past_lam \<Phi> x = Some y \<Longrightarrow> inv_map_past_lam \<Phi>' y = Some x"
+  by (cases x) auto
+
+lemma inv_inv_map_past_lam_inv [simp]: "(\<And>x y. \<Phi> x = Some y \<Longrightarrow> \<Phi>' y = Some x) \<Longrightarrow> 
+    inv_map_past_lam \<Phi> x = Some y \<Longrightarrow> map_past_lam \<Phi>' y = Some x"
+  by (cases x) (auto split: nat.splits)
+
+lemma inv_map_past_let_inv [simp]: "(\<And>x y. \<Phi> x = Some y \<Longrightarrow> \<Phi>' y = Some x) \<Longrightarrow> 
+    map_past_let \<Phi> x = Some y \<Longrightarrow> inv_map_past_let \<Phi>' y = Some x"
+  by (cases x) auto
+
+lemma inv_inv_map_past_let_inv [simp]: "(\<And>x y. \<Phi> x = Some y \<Longrightarrow> \<Phi>' y = Some x) \<Longrightarrow> 
+    inv_map_past_let \<Phi> x = Some y \<Longrightarrow> map_past_let \<Phi>' y = Some x"
+  by (cases x) (auto split: if_splits)
+
+lemma dom_map_past_lam [simp]: "dom (map_past_lam \<Phi>) = insert 0 (Suc ` dom \<Phi>)"
+proof (auto simp add: dom_def split: nat.splits)
+  fix x
+  show "x \<notin> Suc ` {a. \<exists>aa b. \<Phi> a = Some (aa, b)} \<Longrightarrow> 
+    \<forall>x2. x = Suc x2 \<longrightarrow> (\<exists>b a. \<Phi> x2 = Some (a, b)) \<Longrightarrow> x = 0" by (cases x) auto
+qed
+
+lemma dom_map_past_let [simp]: "dom (map_past_let \<Phi>) = insert 0 (Suc ` dom \<Phi>)"
+proof (auto simp add: dom_def split: nat.splits)
+  fix x
+  show "x \<notin> Suc ` {a. \<exists>aa b. \<Phi> a = Some (aa, b)} \<Longrightarrow>
+    \<forall>x2. x = Suc x2 \<longrightarrow> (\<exists>a b. \<Phi> x2 = Some (a, b)) \<Longrightarrow> x = 0" by (cases x) auto
+qed
+
+lemma dom_inv_map_past_lam [simp]: "dom (inv_map_past_lam \<Phi>) = insert (0, 0) (apfst Suc ` dom \<Phi>)"
+  by (auto simp add: dom_def image_iff split: nat.splits) force+
+
+lemma dom_inv_map_past_let [simp]: "dom (inv_map_past_let \<Phi>) = 
+    insert (0, 0) ((\<lambda>(x, y). (x, if x = 0 then Suc y else y)) ` dom \<Phi>)"
+  by (auto simp add: dom_def image_iff split: if_splits)
+     (force, metis Suc_pred not_None_eq, force)
+
+lemma combine_split_cancel' [simp]: "\<Gamma> \<turnstile>\<^sub>d e : t \<Longrightarrow> dom \<Phi> = dom (lookup \<Gamma>) \<Longrightarrow> 
+  (\<And>x y. \<Phi> x = Some y \<Longrightarrow> \<Phi>' y = Some x) \<Longrightarrow> combine_vars' \<Phi>' (split_vars' \<Phi> e) = e"
+proof (induction \<Gamma> e t arbitrary: \<Phi> \<Phi>' rule: typing\<^sub>d.induct)
+  case (tc\<^sub>d_var \<Gamma> x t)
+  moreover hence "x \<in> dom \<Phi>" by auto
+  ultimately show ?case by fastforce
+next
+  case (tc\<^sub>d_lam t\<^sub>1 \<Gamma> e t\<^sub>2)
+  moreover hence "\<And>x y. map_past_lam \<Phi> x = Some y \<Longrightarrow> inv_map_past_lam \<Phi>' y = Some x"
+    using inv_map_past_lam_inv by fastforce
+  ultimately show ?case by (simp add: Let_def)
+next
+  case (tc\<^sub>d_let \<Gamma> e\<^sub>1 t\<^sub>1 e\<^sub>2 t\<^sub>2)
+  moreover hence "\<And>x y. map_past_let \<Phi> x = Some y \<Longrightarrow> inv_map_past_let \<Phi>' y = Some x" 
+    using inv_map_past_let_inv by fastforce
+  ultimately show ?case by simp
+qed simp_all
+     
+lemma combine_split_cancel [simp]: "[] \<turnstile>\<^sub>d e : t \<Longrightarrow> combine_vars (split_vars e) = e"
+proof (unfold combine_vars_def split_vars_def)
+  assume "[] \<turnstile>\<^sub>d e : t" 
+  moreover have "dom Map.empty = dom (lookup [])" by simp
+  moreover have "\<And>x y. Map.empty x = Some y \<Longrightarrow> Map.empty y = Some x" by simp
+  ultimately show "combine_vars' Map.empty (split_vars' Map.empty e) = e" 
+    by (metis combine_split_cancel')
+qed
+
+lemma split_combine_cancel' [simp]: "\<Gamma> \<turnstile>\<^sub>g e : t \<Longrightarrow> (\<And>x y. \<Phi> x = Some y \<Longrightarrow> \<Phi>' y = Some x) \<Longrightarrow>  
+  dom \<Phi> = {xy. \<exists>z. lookup \<Gamma> (fst xy) = Some z \<and> snd xy \<in> dom (lookup z)} \<Longrightarrow>
+  split_vars' \<Phi>' (combine_vars' \<Phi> e) = e"
+proof (induction \<Gamma> e t arbitrary: \<Phi> \<Phi>' rule: typing\<^sub>g.induct)
+  case (tc\<^sub>g_var \<Gamma> x ts y t)
+  hence "(x, y) \<in> dom \<Phi>" by auto
+  with tc\<^sub>g_var show ?case by fastforce
+next
+  case (tc\<^sub>g_lam t\<^sub>1 \<Gamma> e t\<^sub>2)
+  hence X: "\<And>x y. inv_map_past_lam \<Phi> x = Some y \<Longrightarrow> map_past_lam \<Phi>' y = Some x" 
+    using inv_inv_map_past_lam_inv by fastforce
+  have Y: "insert_at 0 [t\<^sub>1] \<Gamma> \<noteq> []" by (cases \<Gamma>) simp_all
+  have "\<And>xy. (xy = (0, 0) \<or> 
+    (\<exists>a b. (\<exists>z. lookup \<Gamma> a = Some z \<and> b \<in> dom (lookup z)) \<and> xy = (Suc a, b))) =
+    (\<exists>z. lookup ([t\<^sub>1] # \<Gamma>) (fst xy) = Some z \<and> snd xy \<in> dom (lookup z))" 
+  proof 
+    fix xy
+    assume "\<exists>z. lookup ([t\<^sub>1] # \<Gamma>) (fst xy) = Some z \<and> snd xy \<in> dom (lookup z)"
+    moreover obtain x y where X: "xy = (x, y)" by fastforce
+    ultimately obtain z where "lookup ([t\<^sub>1] # \<Gamma>) x = Some z \<and> y \<in> dom (lookup z)" by auto
+    with X show "xy = (0, 0) \<or> 
+      (\<exists>a b. (\<exists>z. lookup \<Gamma> a = Some z \<and> b \<in> dom (lookup z)) \<and> xy = (Suc a, b))" 
+        by (cases x, cases y) auto
+  qed auto
+  with tc\<^sub>g_lam have "\<And>xy. xy \<in> insert (0, 0) (apfst Suc ` dom \<Phi>) =
+    (xy \<in> {xy. \<exists>z. lookup (insert_at 0 [t\<^sub>1] \<Gamma>) (fst xy) = Some z \<and> snd xy \<in> dom (lookup z)})" 
+      by (cases \<Gamma>) (simp_all add: image_iff)
+  hence "insert (0, 0) (apfst Suc ` dom \<Phi>) =
+    {xy. \<exists>z. lookup (insert_at 0 [t\<^sub>1] \<Gamma>) (fst xy) = Some z \<and> snd xy \<in> dom (lookup z)}" 
+    by (rule set_eqI)
+  with tc\<^sub>g_lam X Y show ?case by (simp add: Let_def)
+next
+  case (tc\<^sub>g_let \<Gamma> e\<^sub>1 t\<^sub>1 e\<^sub>2 t\<^sub>2)
+  hence X: "\<And>x y. inv_map_past_let \<Phi> x = Some y \<Longrightarrow> map_past_let \<Phi>' y = Some x" 
+    using inv_inv_map_past_let_inv by fastforce
+
+  from tc\<^sub>g_let have "\<Gamma> \<turnstile>\<^sub>g e\<^sub>1 : t\<^sub>1" by simp
+  from tc\<^sub>g_let have "cons_fst t\<^sub>1 \<Gamma> \<turnstile>\<^sub>g e\<^sub>2 : t\<^sub>2" by simp
+  from tc\<^sub>g_let have "split_vars' \<Phi>' (combine_vars' \<Phi> e\<^sub>1) = e\<^sub>1" by simp
+  from tc\<^sub>g_let have "\<Phi> xx = Some xy \<Longrightarrow> \<Phi>' xy = Some xx" by simp
+  from tc\<^sub>g_let have "dom \<Phi> = {xy. \<exists>z. lookup \<Gamma> (fst xy) = Some z \<and> snd xy \<in> dom (lookup z)}" by simp
+
+
+  have Y: "\<And>xy. xy \<in> insert (0, 0) ((\<lambda>x. case x of (x, y) \<Rightarrow> (x, if x = 0 then Suc y else y)) `
+    {xy. \<exists>z. lookup \<Gamma> (fst xy) = Some z \<and> snd xy \<in> dom (lookup z)}) \<Longrightarrow>
+    xy \<in> {xy. \<exists>z. (case fst xy of 0 \<Rightarrow> (case lookup \<Gamma> 0 of None \<Rightarrow> Some [t\<^sub>1] 
+      | Some aa \<Rightarrow> Some (t\<^sub>1 # aa)) | Suc x' \<Rightarrow> lookup \<Gamma> (fst xy)) = Some z \<and> 
+      snd xy \<in> dom (lookup z)}" 
+    by (auto simp add: image_iff split: option.splits nat.splits)
+  have "\<And>xy. xy \<in> {xy. \<exists>z. (case fst xy of 0 \<Rightarrow> (case lookup \<Gamma> 0 of None \<Rightarrow> Some [t\<^sub>1] 
+      | Some aa \<Rightarrow> Some (t\<^sub>1 # aa)) | Suc x' \<Rightarrow> lookup \<Gamma> (fst xy)) = Some z \<and> 
+      snd xy \<in> dom (lookup z)} \<Longrightarrow> 
+    xy \<in> insert (0, 0) ((\<lambda>x. case x of (x, y) \<Rightarrow> (x, if x = 0 then Suc y else y)) `
+      {xy. \<exists>z. lookup \<Gamma> (fst xy) = Some z \<and> snd xy \<in> dom (lookup z)})" 
+  proof
+    fix xy
+    assume "xy \<in> {xy. \<exists>z. (case fst xy of 0 \<Rightarrow> (case lookup \<Gamma> 0 of None \<Rightarrow> Some [t\<^sub>1] 
+      | Some aa \<Rightarrow> Some (t\<^sub>1 # aa)) | Suc x' \<Rightarrow> lookup \<Gamma> (fst xy)) = Some z \<and>
+        snd xy \<in> dom (lookup z)}"
+    moreover assume "xy \<notin> (\<lambda>x. case x of (x, y) \<Rightarrow> (x, if x = 0 then Suc y else y)) `
+      {xy. \<exists>z. lookup \<Gamma> (fst xy) = Some z \<and> snd xy \<in> dom (lookup z)}"
+    moreover obtain x y where "xy = (x, y)" by fastforce
+    ultimately show "xy = (0, 0)" by (auto simp add: image_iff split: nat.splits option.splits)
+  qed
+  with Y have "insert (0, 0) ((\<lambda>x. case x of (x, y) \<Rightarrow> (x, if x = 0 then Suc y else y)) `
+    {xy. \<exists>z. lookup \<Gamma> (fst xy) = Some z \<and> snd xy \<in> dom (lookup z)}) =
+    {xy. \<exists>z. (case fst xy of 0 \<Rightarrow> (case lookup \<Gamma> 0 of None \<Rightarrow> Some [t\<^sub>1] | Some aa \<Rightarrow> Some (t\<^sub>1 # aa))
+      | Suc x' \<Rightarrow> lookup \<Gamma> (fst xy)) = Some z \<and> snd xy \<in> dom (lookup z)}" 
+    by blast
+  with tc\<^sub>g_let X show ?case by simp
+qed simp_all
+
+lemma split_combine_cancel [simp]: "[] \<turnstile>\<^sub>g e : t \<Longrightarrow> split_vars (combine_vars e) = e"
+proof (unfold combine_vars_def split_vars_def)
+  assume "[] \<turnstile>\<^sub>g e : t"
+  moreover have "\<And>x y. Map.empty x = Some y \<Longrightarrow> Map.empty y = Some x" by simp 
+  moreover have "dom Map.empty = {xy. \<exists>z. lookup [] (fst xy) = Some z \<and> snd xy \<in> dom (lookup z)}" 
+    using lookup.elims option.simps(3) by force
+  ultimately show "split_vars' Map.empty (combine_vars' Map.empty e) = e"
+    by (rule split_combine_cancel')
+qed
+
+text \<open>Now, we can define our combining function on closures, callstacks, and states. The 
+environments contained in the closures, which caused so much difficulties the other way around, are 
+simply concatenated together.\<close>
+
+fun map_from_env :: "'a list list \<Rightarrow> nat \<times> nat \<rightharpoonup> nat" where
+  "map_from_env [] (x, y) = None"
+| "map_from_env (cs # \<Delta>) (0, y) = (if y < length cs then Some y else None)"
+| "map_from_env (cs # \<Delta>) (Suc x, y) = map_option ((+) (length cs)) (map_from_env \<Delta> (x, y))"
+
+lemma lookup_map_from_env [simp]: "lookup \<Delta> x = Some cs \<Longrightarrow> lookup cs y = Some c \<Longrightarrow> 
+    map_from_env \<Delta> (x, y) \<noteq> None"
+  by (induction \<Delta> "(x, y)" arbitrary: x y rule: map_from_env.induct) simp_all
+
+lemma lookup_concat_map_from_env [simp]: "lookup \<Delta> x = Some cs \<Longrightarrow> lookup cs y = Some c \<Longrightarrow> 
+    lookup (concat \<Delta>) (the (map_from_env \<Delta> (x, y))) = Some c"
+proof (induction \<Delta> "(x, y)" arbitrary: x y rule: map_from_env.induct)
+  case (3 cs \<Delta> x y)
+  then show ?case by (cases "map_from_env \<Delta> (x, y)") simp_all
+qed simp_all
+
+primrec combine_closure :: "closure\<^sub>g \<Rightarrow> closure\<^sub>c" where
+  "combine_closure (Num\<^sub>g n) = Const\<^sub>c n"
+| "combine_closure (Fun\<^sub>g t \<Delta> e n) = 
+    Lam\<^sub>c t (concat (map (map combine_closure) \<Delta>)) 
+      (combine_vars' (inv_map_past_lam (map_from_env \<Delta>)) e)"
+
+primrec combine_frame :: "frame\<^sub>g \<Rightarrow> frame\<^sub>c" where
+  "combine_frame (FApp1\<^sub>g \<Delta> e) = 
+    FApp1\<^sub>c (concat (map (map combine_closure) \<Delta>)) (combine_vars' (map_from_env \<Delta>) e)"
+| "combine_frame (FApp2\<^sub>g c) = FApp2\<^sub>c (combine_closure c)"
+| "combine_frame (FLet\<^sub>g \<Delta> e) = 
+    FLet\<^sub>c (concat (map (map combine_closure) \<Delta>)) (combine_vars' (map_from_env \<Delta>) e)"
+| "combine_frame (FPop\<^sub>g c) = FPop\<^sub>c (combine_closure c)"
+| "combine_frame (FReturn\<^sub>g \<Delta>) = FReturn\<^sub>c (concat (map (map combine_closure) \<Delta>))"
+
+primrec combine_state :: "state\<^sub>g \<Rightarrow> state\<^sub>c" where
+  "combine_state (SE\<^sub>g s \<Delta> e) = 
+    SE\<^sub>c (map combine_frame s) (concat (map (map combine_closure) \<Delta>)) 
+      (combine_vars' (map_from_env \<Delta>) e)"
+| "combine_state (SC\<^sub>g s c) = SC\<^sub>c (map combine_frame s) (combine_closure c)"
+
+text \<open>We can now prove our typechecking theorems: note again how the "empty" context cannot really 
+be \<open>[]\<close>, because of the need for a space to put top-level lets in.\<close>
+
+lemma map_from_env_insert' [simp]: "map_from_env (insert_at 0 [t] \<Gamma>) x = 
+    inv_map_past_lam (map_from_env \<Gamma>) x"
+  by (induction \<Gamma> x rule: map_from_env.induct) (simp_all split: nat.splits)
+
+lemma map_from_env_insert [simp]: "map_from_env (insert_at 0 [t] \<Gamma>) = 
+    inv_map_past_lam (map_from_env \<Gamma>)"
+  by auto
+
+lemma map_from_env_mapfst' [simp]: "map_from_env (cons_fst t \<Gamma>) x = 
+    inv_map_past_let (map_from_env \<Gamma>) x"
+proof (induction \<Gamma> x rule: map_from_env.induct)
+  case (1 x y)
+  thus ?case by (cases x) simp_all
+qed (auto simp add: option.map_comp)
+
+lemma map_from_env_mapfst [simp]: "map_from_env (cons_fst t \<Gamma>) = inv_map_past_let (map_from_env \<Gamma>)"
+  by auto
+
+lemma typecheck_combine [simp]: "\<Gamma> \<turnstile>\<^sub>g e : t \<Longrightarrow> concat \<Gamma> \<turnstile>\<^sub>d combine_vars' (map_from_env \<Gamma>) e : t"
+  by (induction \<Gamma> e t rule: typing\<^sub>g.induct) simp_all
+
+lemma "c :\<^sub>g\<^sub>c\<^sub>l t \<Longrightarrow> True"
+  and map_from_env_type_vals' [simp]: "\<Delta> :\<^sub>g\<^sub>c\<^sub>l\<^sub>s \<Gamma> \<Longrightarrow> map_from_env \<Gamma> x = map_from_env \<Delta> x"
+proof (induction c t and \<Delta> \<Gamma> arbitrary: and x rule: typing_closure\<^sub>g_typing_environment\<^sub>g.inducts)
+  case tc\<^sub>c_nil
+  thus ?case by (cases x) simp_all
+next
+  case (tc\<^sub>c_cons_nil \<Delta> \<Gamma>)
+  thus ?case
+  proof (induction x)
+    case (Pair a b)
+    then show ?case by (cases a) simp_all
+  qed
+next
+  case (tc\<^sub>c_cons_cons c t cs \<Delta> ts \<Gamma>)
+  thus ?case 
+  proof (induction x)
+    case (Pair a b)
+    hence Y: "length cs = length ts" by simp
+    hence "map_from_env ((t # ts) # \<Gamma>) (a, b) = map_from_env ((c # cs) # \<Delta>) (a, b)" 
+    proof (cases a)
+      case (Suc a)
+      from Pair have "map_from_env (ts # \<Gamma>) (Suc a, b) = map_from_env (cs # \<Delta>) (Suc a, b)" by blast
+      with Y Suc show ?thesis 
+        by (cases "map_from_env \<Gamma> (a, b)", simp, cases "map_from_env \<Delta> (a, b)") simp_all
+    qed simp_all
+    thus ?case by simp
+  qed
+qed simp_all
+
+lemma map_from_env_type_vals [simp]: "\<Delta> :\<^sub>g\<^sub>c\<^sub>l\<^sub>s \<Gamma> \<Longrightarrow> map_from_env \<Gamma> = map_from_env \<Delta>"
+  by auto
+
+lemma typecheck_combine_closure [simp]: "c :\<^sub>g\<^sub>c\<^sub>l t \<Longrightarrow> combine_closure c :\<^sub>c\<^sub>l t"
+  and typecheck_concat_combine_closure [simp]: "\<Delta> :\<^sub>g\<^sub>c\<^sub>l\<^sub>s \<Gamma> \<Longrightarrow> 
+    concat (map (map combine_closure) \<Delta>) :\<^sub>c\<^sub>l\<^sub>s concat \<Gamma>"
+proof (induction c t and \<Delta> \<Gamma> rule: typing_closure\<^sub>g_typing_environment\<^sub>g.inducts)
+  case (tc\<^sub>c_lam \<Delta> \<Gamma> t\<^sub>1 e t\<^sub>2)
+  hence X: "map_from_env \<Gamma> = map_from_env \<Delta>" by simp
+  from tc\<^sub>c_lam have "concat (insert_at 0 [t\<^sub>1] \<Gamma>) \<turnstile>\<^sub>d 
+    combine_vars' (map_from_env (insert_at 0 [t\<^sub>1] \<Gamma>)) e : t\<^sub>2" by (metis typecheck_combine)
+  hence "insert_at 0 t\<^sub>1 (concat \<Gamma>) \<turnstile>\<^sub>d combine_vars' (inv_map_past_lam (map_from_env \<Gamma>)) e : t\<^sub>2" 
+    by simp
+  hence "insert_at 0 t\<^sub>1 (concat \<Gamma>) \<turnstile>\<^sub>d combine_vars' (inv_map_past_lam (map_from_env \<Delta>)) e : t\<^sub>2" 
+    using X by metis
+  with tc\<^sub>c_lam show ?case by simp
+qed simp_all
+
+lemma combine_clsoure_mapfst [simp]: "concat (map (map combine_closure) (cons_fst c \<Delta>)) = 
+    combine_closure c # concat (map (map combine_closure) \<Delta>)"
+  by (induction \<Delta>) simp_all
+
+lemma latest_combine_env [simp]: "latest_environment\<^sub>c (map combine_frame s) =
+  map_option (\<lambda>\<Delta>. concat (map (map combine_closure) \<Delta>)) (latest_environment\<^sub>g s)"
+proof (induction s rule: latest_environment\<^sub>g.induct)
+  case (5 c s)
+  then show ?case by (simp add: option.map_comp comp_def)
+qed simp_all
+
+lemma typecheck_stack [simp]: "s :\<^sub>g t\<^sub>2 \<rightarrow> t \<Longrightarrow> map combine_frame s :\<^sub>c t\<^sub>2 \<rightarrow> t"
+proof (induction s t\<^sub>2 t rule: typing_stack\<^sub>g.induct)
+  case (tcc_scons_app1 \<Delta> \<Gamma> e t\<^sub>1 s t\<^sub>2 t)
+  hence X: "concat (map (map combine_closure) \<Delta>) :\<^sub>c\<^sub>l\<^sub>s concat \<Gamma>" by simp
+  from tcc_scons_app1 have "map_from_env \<Delta> = map_from_env \<Gamma>" by simp
+  with tcc_scons_app1(2) have Y: "concat \<Gamma> \<turnstile>\<^sub>d combine_vars' (map_from_env \<Delta>) e : t\<^sub>1" by simp
+  from tcc_scons_app1 have "latest_environment\<^sub>c (map combine_frame s) = 
+    Some (concat (map (map combine_closure) \<Delta>))" by simp
+  with tcc_scons_app1 X Y have "FApp1\<^sub>c (concat (map (map combine_closure) \<Delta>)) 
+    (combine_vars' (map_from_env \<Delta>) e) # map combine_frame s :\<^sub>c Arrow t\<^sub>1 t\<^sub>2 \<rightarrow> t" 
+      by (metis typing_stack\<^sub>c.tcc_scons_app1)
+  thus ?case by simp
+next
+  case (tcc_scons_app2 c t\<^sub>1 t\<^sub>2 s t)
+  then show ?case by simp
+next
+  case (tcc_scons_let s \<Delta> \<Gamma> t\<^sub>1 e t\<^sub>2 t)
+  then show ?case by simp
+next
+  case (tcc_scons_pop s \<Delta> c tt t' t)
+  then show ?case by simp
+next
+  case (tcc_scons_ret \<Delta> \<Gamma> s t' t)
+  then show ?case by simp
+qed simp_all
+                                  
+end
